Fix whole_prog proof and remove news-printing option
After discussion with @myreen and the Pancake meeting, printing the
entirety of `NEWS.md` has the unfortunate side effect of storing a
~15kb (and growing) string in memory, that needs to be copied over
every time the GC runs.

Therefore, this commit keeps only the `--pancake_feature=T` query
and drops the option to print `NEWS.md.` The usage notes instead
explain where the news can be found.

pancake/newsScript.sml
@@ -13,10 +13,6 @@ val news_in = openIn "NEWS.md";
 val news = inputAll news_in;
 val _ = closeIn news_in;
 
-Definition news_def:
-  news = ^(toMLstring news)
-End
-
 val aprefix = "<sub>"
 val eprefix = "<sub>Feature enabled: `"
 val dprefix = "<sub>Feature disabled: `"
