compiler/bootstrap/translation/compiler64ProgScript.sml
@@ -428,9 +428,7 @@ val res = translate (has_help_flag_def |> SIMP_RULE (srw_ss()) [MEMBER_INTRO])
 val res = translate print_option_def
 val res = translate current_build_info_str_def
 val res = translate compilerTheory.help_string_def;
-val res = translate newsTheory.news_def
 val res = translate (newsTheory.query_news_def |> SIMP_RULE (srw_ss()) [MEMBER_INTRO])
-val res = translate (has_pancake_news_flag_def |> SIMP_RULE (srw_ss()) [MEMBER_INTRO])
 val res = translate parse_pancake_feature_def
 val res = translate print_bool_def
 
@@ -648,8 +646,6 @@ Quote add_cakeml:
       print compiler_help_string
     else if compiler_has_version_flag cl then
       print compiler_current_build_info_str
-    else if compiler_has_pancake_news_flag cl then
-      print news_news
     else
       case compiler_parse_pancake_feature cl of
         Some rest => print (compiler_print_bool(news_query_news rest))
@@ -668,7 +664,6 @@ End
 val main_v_def = fetch "-" "main_v_def";
 val compiler_help_string_v_thm = fetch "-" "compiler_help_string_v_thm";
 val compiler_current_build_info_str_v_thm = fetch "-" "compiler_current_build_info_str_v_thm";
-val news_news_v_thm = fetch "-" "news_news_v_thm";
 
 Theorem main_spec:
   ¬has_repl_flag (TL cl) ∧ IS_SOME (stdin_content fs) ⇒
@@ -732,14 +727,6 @@ Proof
     \\ CONV_TAC SWAP_EXISTS_CONV
     \\ qexists_tac`fs`
     \\ xsimpl)
-  \\ xlet_auto>-xsimpl
-  \\ xif
-  >- (simp[full_compile_64_def]
-      \\ xapp
-      \\ irule_at (Pos hd) news_news_v_thm
-      \\ xsimpl
-      \\ qexists_tac`fs`
-      \\ xsimpl)
   \\ xlet_auto >- xsimpl
   \\ gvs[oneline std_preludeTheory.OPTION_TYPE_def]
   \\ reverse PURE_FULL_CASE_TAC
@@ -832,9 +819,12 @@ Proof
   \\ qmatch_goalsub_abbrev_tac`fs1 = _ with numchars := _`
   \\ qexists_tac`fs1`
   \\ reverse conj_tac >-
-   rw[Abbr`fs1`,full_compile_64_def,UNCURRY,
-      GSYM fastForwardFD_with_numchars,
-      GSYM add_stdo_with_numchars, with_same_numchars]
+   (rw[Abbr`fs1`,full_compile_64_def,UNCURRY,
+       GSYM fastForwardFD_with_numchars,
+       GSYM add_stdo_with_numchars, with_same_numchars]
+    \\ PURE_FULL_CASE_TAC
+    \\ rw[GSYM fastForwardFD_with_numchars,
+          GSYM add_stdo_with_numchars, with_same_numchars, UNCURRY])
   \\ simp [SEP_CLAUSES]
   \\ match_mp_tac (MP_CANON(MATCH_MP app_wgframe (UNDISCH main_spec)))
   \\ xsimpl
